rename bloom_filter_alt to bloom_filter

theories/coneris/examples/bloom_filter/concurrent_bloom_filter.v
@@ -1,161 +1,284 @@
 From iris.base_logic.lib Require Import invariants.
 From iris.algebra Require Import gset_bij auth excl frac agree numbers.
-From clutch.coneris Require Import coneris par spawn spin_lock hash atomic lock concurrent_hash con_hash_interface1 bloom_filter.
+From clutch.coneris Require Import
+  coneris par spawn spin_lock hash atomic lock
+  con_hash_interface4 bloom_filter.
 From clutch.coneris.lib Require Import list array.
 
 Set Default Proof Using "Type*".
 
-(*
-
 Section conc_bloom_filter.
+  Variables filter_size max_key num_hash : nat.
+  Context `{!conerisGS Σ, !spawnG Σ,
+      c : con_hash4 Σ,
+      !inG Σ (excl_authR boolO), !inG Σ (prodR fracR val0) }.
 
-
-
-  Variables filter_size num_hash num_threads : nat.
-  Context `{!conerisGS Σ, !spawnG Σ, c:con_hash1 Σ filter_size, !inG Σ (excl_authR boolO), !inG Σ (prodR fracR val0) }.
-
-
-  Definition init_bloom_filter : expr :=
+  Definition init_bloom_filter : val :=
     λ: "_" ,
-      let: "hfuns" := list_seq_fun #0 #num_hash
-                        (λ: "_", let: "h" := init_hash1 #() in
-                                 let: "α" := allocate_tape1 #() in
-                                 ("h", "α"))%E in
+      let: "hfuns" := list_seq_fun #0 #num_hash (λ: "_", init_con_hash #filter_size #max_key) in
       let: "arr" := array_init #(S filter_size) (λ: "x", #false)%E in
       let: "l" := ref ("hfuns", "arr") in
       "l".
 
-  Definition insert_bloom_filter : expr :=
+  Definition insert_bloom_filter : val :=
     λ: "l" "v" ,
       let, ("hfuns", "arr") := !"l" in
-      list_iter (λ: "ht",
-          let, ("h", "α") := "ht" in
-          let: "i" := "h" "v" "α" in
+      list_iter (λ: "h",
+          let: "i" := "h" "v" in
           "arr" +ₗ "i" <- #true) "hfuns".
 
-
-  Definition lookup_bloom_filter : expr :=
+  Definition lookup_bloom_filter : val :=
     λ: "l" "v" ,
       let, ("hfuns", "arr") := !"l" in
       let: "res" := ref #true in
-      list_iter (λ: "ht",
-          let, ("h", "α") := "ht" in
-          let: "i" := "h" "v" "α" in
+      list_iter (λ: "h",
+          let: "i" := "h" "v" in
           if: !("arr" +ₗ "i") then #() else "res" <- #false) "hfuns" ;;
       !"res".
 
-(*
-  (*
-     The invariant of the case study keeps track of three sets, s1, s2, and s3, whose union s is always constant.
-       - s1 represents the set of elements that are in the tape of some hash
-       - s2 represents the set of indices that have been read from the hash, but are still waiting to be written to
-       the array
-       - s3 represents the set of indices of the array that have been set to 1
+  Definition insert_bloom_filter_loop : val :=
+    (rec: "aux" "bfl" "ks" :=
+       match: "ks" with
+         NONE => #()
+       | SOME "p" =>
+           let: "h" := Fst "p" in
+           let: "t" := Snd "p" in
+           (insert_bloom_filter "bfl" "h") ||| ("aux" "bfl" "t")
+       end).
 
-     After the initialization, s1 will contain all elements in the hash sets, while s2 and s3 are empty. The deterministic
-     part of the program will just advance the physical state of the bloom filter so that at the end s1 and s2 are empty.
-
-     Additionally, the invariant ensures that every thread reading from a hash will find a non-empty tape (and therefore there
-     is no more sampling happening).
-   *)
-  Definition bloom_filter_inv (s : gset nat) (a : loc) (arr lbls : list val) (snames : list hash_set_gname) (tnames : list hash_tape_gname): iProp Σ :=
-    ∃ (s1 s2 s3 : gset nat),
-      ⌜ s1 ∪ s2 ∪ s3 = s ⌝ ∗
-      (* Every element in s1 is in the tape of some hash *)
-      ([∗ list] x ∈ (zip lbls (zip snames tnames)),
-           ∃ (sx : list nat), hash_tape1 (fst x) sx (fst (snd x)) (snd (snd x)) ∗ ⌜ subseteq (list_to_set sx) s1 ⌝) ∗
-      (* Every element in s2 is waiting to be written *)
-      (* Every element in s3 is an index set to 1 in the array *)
-      (a ↦∗ arr) ∗
-      ⌜ forall i, arr !! i = Some #true -> i ∈ s3  ⌝ ∗
-      ⌜ forall i, i ∈ s3 -> (i < S filter_size)%nat  ⌝ ∗
-      ([∗ set] x ∈ s3, ∃ γ, (hash_set_frag1 x γ)).
- *)
-
-  Variable hash_tape_token : val -> nat -> hash_tape_gname -> iProp Σ.
-  Lemma hash_token_non_empty α ns k γ1 γ2 :
-    hash_tape1 α ns γ1 γ2 -∗ hash_tape_token α (S k) γ2 -∗
-   ⌜ exists n ns', ns = n :: ns' ⌝.
-  Admitted.
-
-  Lemma hash_token_combine α k k' γ2 :
-    hash_tape_token α k γ2 ∗ hash_tape_token α k' γ2 ⊣⊢ hash_tape_token α (k + k') γ2.
-  Admitted.
-
-  Lemma hash_frag_valid k v γ γ2 :
-    hash_frag1 k v γ γ2 -∗ ⌜ (v ≤ filter_size)%nat ⌝.
-  Admitted.
+  Definition main_bloom_filter (ksv ktest : val) : expr :=
+      let: "bfl" := init_bloom_filter #() in
+      insert_bloom_filter_loop "bfl" ksv ;;
+      lookup_bloom_filter "bfl" ktest.
 
 
-  Definition con_hash_inv_list N hfs hnames :=
-      ([∗ list] k↦hf;γ ∈ hfs;hnames,
-        ∃ f α lk hm ns,
-          ⌜ hf = (f, α)%V ⌝ ∗
-          hash_tape1 α ns γ.2.1 γ.2.2.1 ∗
-        con_hash_inv1 N f lk hm (λ _, True) γ.1 γ.2.1 γ.2.2.1 γ.2.2.2)%I.
+  Definition insert_bloom_filter_loop_seq : val :=
+    (rec: "aux" "bfl" "ks" :=
+       match: "ks" with
+         NONE => #()
+       | SOME "p" =>
+           let: "h" := Fst "p" in
+           let: "t" := Snd "p" in
+           (insert_bloom_filter "bfl" "h") ;; ("aux" "bfl" "t")
+       end).
+
+  Definition main_bloom_filter_seq (ksv ktest : val) : expr :=
+      let: "bfl" := init_bloom_filter #() in
+      insert_bloom_filter_loop_seq "bfl" ksv ;;
+      lookup_bloom_filter "bfl" ktest.
 
 
-  Lemma con_hash_inv_list_cons N hf hfs2 hnames :
-    con_hash_inv_list N ((hf :: hfs2)) hnames -∗
-    (∃ f α lk hm γ hnames2 ns,
-        ⌜ hf = (f, α)%V⌝ ∗ ⌜ hnames = γ :: hnames2 ⌝ ∗
-         hash_tape1 α ns γ.2.1 γ.2.2.1 ∗
-         con_hash_inv1 N f lk hm (λ _, True) γ.1 γ.2.1 γ.2.2.1 γ.2.2.2 ∗
-         con_hash_inv_list N hfs2 hnames2
-    ).
-  Admitted.
+  Definition con_hash_inv_list hfs hnames ks (s : gset nat) :=
+    ([∗ list] i ↦f;γ ∈ hfs;hnames,
+       conhashfun γ filter_size f ∗
+       ([∗ list] k ∈ ks, ∃ n, ⌜ n ∈ s ⌝ ∗ hashkey γ k (Some n)))%I.
 
-
-
-  Definition bloom_filter_inv N bfl hfuns a
-    (hnames : list (hash_view_gname * (hash_set_gname * (hash_tape_gname * hash_lock_gname)))) (s : gset nat) : iPropI Σ :=
-      inv (N.@"bf")
-        (∃ hfs,
-          (bfl ↦ (hfuns, LitV (LitLoc a))%V ∗
-          ⌜ is_list_HO hfs hfuns ⌝ ∗
-          ⌜ length hfs = num_hash ⌝ ∗
-          con_hash_inv_list N hfs hnames ∗
-          ⌜ forall i, i ∈ s -> (i < S filter_size)%nat  ⌝ ∗
-          (∃ (arr : list val),
-            (a ↦∗ arr) ∗
-            ⌜ length arr = S filter_size ⌝ ∗
-            ⌜ forall i, i < S filter_size -> arr !! i = Some #true -> i ∈ s  ⌝)))%I.
-
-
-  Lemma bloom_filter_init_spec N :
-    {{{ ↯ (fp_error filter_size num_hash (num_hash * num_threads) 0) }}}
-      init_bloom_filter #()
-    {{{ (bfl:loc), RET #bfl ;
-        ∃ hfuns a hnames s,
-        bloom_filter_inv N bfl hfuns a hnames s
-    }}}.
+  Lemma con_hash_inv_list_cons f fs2 hnames ks s :
+    con_hash_inv_list ((f :: fs2)) hnames ks s -∗
+    (∃ γ hnames2,
+        ⌜ hnames = γ :: hnames2 ⌝ ∗
+        conhashfun γ filter_size f∗
+        ([∗ list] k ∈ ks, ∃ n, ⌜ n ∈ s ⌝ ∗ hashkey γ k (Some n)) ∗
+        con_hash_inv_list fs2 hnames2 ks s).
   Proof.
-    iIntros (Φ) "Herr HΦ".
+    iIntros "Hinv_list".
+    rewrite /con_hash_inv_list.
+    destruct hnames as [| γ hnames2]; auto.
+    iDestruct "Hinv_list" as "(? & ?)".
+    by iFrame.
+  Qed.
+
+  Definition bloom_filter_inv_aux bfl hfuns a
+    hnames ks (s : gset nat) : iPropI Σ :=
+        (∃ hfs,
+            (bfl ↦ (hfuns, LitV (LitLoc a))%V ∗
+            ⌜ is_list_HO hfs hfuns ⌝ ∗
+            ⌜ length hfs = num_hash ⌝ ∗
+            con_hash_inv_list hfs hnames ks s ∗
+            ⌜ forall i, i ∈ s -> (i < S filter_size)%nat  ⌝ ∗
+            (∃ (arr : list val),
+                 (a ↦∗ arr) ∗
+                 ⌜ length arr = S filter_size ⌝ ∗
+                 ⌜ forall i, i < S filter_size -> arr !! i = Some #true \/ arr !! i = Some #false⌝ ∗
+                 ⌜ forall i, i < S filter_size -> arr !! i = Some #true -> i ∈ s  ⌝)))%I.
+
+  Definition bloom_filter_inv N bfl hfuns a hnames ks (s : gset nat) : iPropI Σ :=
+    inv (N.@"bf") (bloom_filter_inv_aux bfl hfuns a hnames ks s).
+
+  Lemma hash_preview_list rem (ks : list nat) f γs (bad : gset nat) :
+     (forall x : nat, x ∈ bad -> (x < S filter_size)%nat) ->
+     conhashfun γs filter_size f -∗
+     ⌜ NoDup ks ⌝ -∗
+     ([∗ list] k ∈ ks, hashkey γs k None) -∗
+     ↯ (fp_error filter_size num_hash (rem + length ks) (size bad)) -∗
+     state_update ⊤ ⊤ (∃ (res : gset nat),
+          ⌜ forall x : nat, x ∈ (bad ∪ res) -> (x < S filter_size)%nat ⌝ ∗
+          ↯ (fp_error filter_size num_hash rem (size (bad ∪ res))) ∗
+          ([∗ list] k ∈ ks, ∃ n, ⌜ n ∈ (bad ∪ res) ⌝ ∗ hashkey γs k (Some n) )).
+  Proof.
+    iIntros (Hbound) "#Hhinv".
+    iInduction ks as [|k ks] "IH" forall (bad Hbound).
+    - iIntros "Hndup Hnone Herr".
+      rewrite /= Nat.add_0_r.
+      iModIntro.
+      iExists bad.
+      replace (bad ∪ bad) with bad by set_solver.
+      iSplit; auto.
+    - iIntros "%Hndup (Hknone & Hksnone) Herr".
+      pose proof (NoDup_cons_1_1 k ks Hndup) as Hdup1.
+      pose proof (NoDup_cons_1_2 k ks Hndup) as Hdup2.
+      replace (rem + length (k :: ks)) with (S rem + (length ks));
+        [|simpl; lia].
+      assert (forall m b, 0 <= fp_error filter_size num_hash m b)%R as Hfp.
+      {
+        intros; apply fp_error_bounded.
+      }
+      iPoseProof (hashkey_presample k bad
+                      (mknonnegreal (fp_error filter_size num_hash (S rem + length ks) (size bad))
+                         (Hfp _ _))
+                      (mknonnegreal (fp_error filter_size num_hash (rem + length ks) (size bad))
+                         (Hfp _ _))
+                      (mknonnegreal (fp_error filter_size num_hash (rem + length ks) (S (size bad)))
+                         (Hfp _ _))
+                      γs with "Hhinv [Hknone] [Herr]") as "Hcur"; auto; try done.
+       + simpl.
+         case_bool_decide.
+         * rewrite fp_error_max /=; auto.
+           rewrite fp_error_max /=; auto.
+           rewrite !Rmult_1_l.
+           lra.
+         * right.
+           rewrite (Rmult_comm (size bad / (filter_size + 1))).
+           rewrite (Rmult_comm ((filter_size + 1 - size bad) / (filter_size + 1))).
+           rewrite Rmult_plus_distr_r.
+           rewrite !(Rmult_assoc _ _ (filter_size + 1)).
+           rewrite !Rinv_l; [lra|].
+           real_solver.
+       + iMod ("Hcur") as "(%v & [(%Hnotbad & Herr)|(%Hbad & Herr)] & Hhauth)"; last first.
+         ** simpl.
+            iMod ("IH" $! bad with "[] [] [Hksnone] [Herr]") as "(%res&?&?&?)"; auto.
+            iModIntro.
+            iExists (bad ∪ res).
+            replace (bad ∪ (bad ∪ res)) with (bad ∪ res) by set_solver.
+            iFrame.
+            iPureIntro.
+            set_solver.
+         ** simpl.
+            iMod ("IH" $! (bad ∪ {[fin_to_nat v]}) with "[] [] [Hksnone] [Herr]") as "(%res&?&?&?)"; auto.
+            *** iPureIntro.
+                intros x Hx.
+                apply elem_of_union in Hx as [Hx|Hx]; auto.
+                apply elem_of_singleton in Hx as ->.
+                apply fin_to_nat_lt.
+            *** rewrite size_union; [|set_solver].
+                rewrite size_singleton.
+                replace (size bad + 1) with (S (size bad)) by lia.
+                iFrame.
+            *** iModIntro.
+                iExists ((bad ∪ {[fin_to_nat v]}) ∪ res).
+                replace (bad ∪ (bad ∪ {[fin_to_nat v]} ∪ res)) with ((bad ∪ {[fin_to_nat v]}) ∪ res) by set_solver.
+                iFrame.
+                iPureIntro.
+                set_solver.
+  Qed.
+
+  Lemma bloom_filter_init_spec N (ks : list nat) :
+    NoDup ks ->
+    ([∗ list] k ∈ ks, ⌜ (k ≤ max_key)%nat ⌝) -∗
+    {{{ ↯ (fp_error filter_size num_hash (num_hash * length ks) 0) }}}
+      init_bloom_filter #()
+   {{{ (bfl:loc), RET #bfl ;
+         ∃ hfuns a hnames s,
+           ↯ (fp_error filter_size num_hash 0 (size s)) ∗
+             ([∗ list] γ ∈ hnames,
+               ([∗ set] k ∈ (set_seq 0 (S max_key) ∖ list_to_set ks), hashkey γ k (None) )) ∗
+             bloom_filter_inv N bfl hfuns a hnames ks s
+   }}}.
+   Proof.
+    iIntros (Hndup) "%Hks".
+    iIntros (Φ).
+    iModIntro.
+    iIntros "Herr HΦ".
     rewrite /init_bloom_filter.
     wp_pures.
-    wp_apply (wp_list_seq_fun_HO _ 0 num_hash _
-                (λ _ fα,
-                  ∃ f α lk hm γ,
-                    ⌜ fα = (f, α)%V ⌝ ∗
-                    hash_set1 ∅ γ.2.1  ∗
-                    hash_tape1 α [] γ.2.1 γ.2.2.1 ∗
-                    con_hash_inv1 N f lk hm (λ _, True) γ.1 γ.2.1 γ.2.2.1 γ.2.2.2)%I).
-    - iIntros (i Ψ).
+    set (Ψ := (λ l, ⌜ num_hash < length l ⌝ ∨
+                (∃ (s : gset nat),
+                      ↯(fp_error filter_size num_hash ((num_hash - length l) * length ks) (size s)) ∗
+                      ⌜ ∀ x : nat, x ∈ s → x < S filter_size ⌝ ∗
+                      ([∗ list] f ∈ l,
+                        (∃ γ,
+                            conhashfun γ filter_size f ∗
+                            ([∗ set] k ∈ (set_seq 0 (S max_key) ∖ list_to_set ks), hashkey γ k (None) ) ∗
+                            ([∗ list] k ∈ ks, ∃ v, ⌜ v ∈ s ⌝ ∗ hashkey γ k (Some v))))))%I).
+    wp_apply (wp_list_seq_fun_HO_invariant _ Ψ
+                0 num_hash _ (λ _ _, True)%I with "[] [Herr] [HΦ]").
+    - iIntros (i l Ξ).
       iModIntro.
-      iIntros "_ HΨ".
+      iIntros "HΨ HΞ".
       wp_pures.
-      wp_apply (con_hash_init1 N (λ _, True)%I); auto.
-      iIntros (f) "(%lk & %hm & %γ1 & %γ2 & %γ3 & %γ4 & #Hinv & Hs)".
-      wp_pures.
-      wp_apply (con_hash_alloc_tape1 with "Hinv").
-      iIntros (α) "Hht".
-      wp_pures.
-      iApply ("HΨ" with "[Hs Hht]").
-      iExists f,α,lk,hm,(γ1,(γ2,(γ3,γ4))).
-      simpl.
+      iApply pgl_wp_state_update.
+      wp_apply conhash_init; auto.
+      iIntros (γ f) "(#Hhinv&Hkeys)".
+      iPoseProof (big_sepS_subseteq with "Hkeys") as "Hkeys".
+      {
+        erewrite (union_difference (list_to_set ks)); [reflexivity|].
+        apply elem_of_subseteq.
+        intros k Hk.
+        apply elem_of_set_seq.
+        split; [lia |].
+        simpl.
+        apply Nat.lt_succ_r.
+        apply elem_of_list_to_set, elem_of_list_lookup in Hk as [? ?].
+        by eapply Hks.
+      }
+      iPoseProof (big_sepS_union with "Hkeys") as "(Hks&Hrest)"; [set_solver|].
+      iPoseProof (big_sepS_list_to_set with "Hks") as "Hks"; auto.
+      iApply "HΞ".
+      iSplitL; auto.
+      rewrite /Ψ cons_length.
+      assert (num_hash ≤ length l \/ num_hash > length l) as [Haux|?] by lia.
+      {
+        iModIntro.
+        iDestruct "HΨ" as "[%|HΨ]"; [iLeft; iPureIntro; lia |].
+        iLeft. iPureIntro. lia.
+      }
+      iDestruct "HΨ" as "[%|HΨ]"; [iModIntro; iLeft; iPureIntro; lia |].
+      iDestruct "HΨ" as "(%s & Herr & %Hbound & Hl)".
+      replace ((num_hash - length l) * length ks) with ((num_hash - S (length l)) * length ks + length ks);
+        last first.
+      {
+        rewrite -{2}(Nat.mul_1_l (length ks)).
+        rewrite -Nat.mul_add_distr_r.
+        f_equal.
+        lia.
+      }
+      iMod (hash_preview_list _ ks _ _ s with "[$][//] Hks Herr") as "Hupd"; auto.
+      iModIntro.
+      iRight.
+      iDestruct "Hupd" as "(%res & ? & Herr & ?)".
+      iExists (s ∪ res).
+      iSplitL "Herr"; auto.
+      iSplit; auto.
+      iApply big_sepL_cons.
       iFrame.
-      iSplit; done.
-    - iIntros (hfuns fαs) "(%Hhfuns & %Hlen & Hinvs)".
+      iSplit; auto.
+      iApply (big_sepL_mono with "Hl").
+      iIntros (k v Hkv) "(%γ'&?&?&?)".
+      iExists γ'.
+      iFrame.
+      iApply (big_sepL_mono with "[$]").
+      iIntros (???) "(%&%&?)".
+      iExists _; iFrame.
+      iPureIntro. set_solver.
+   - rewrite /Ψ.
+     iRight.
+     iExists ∅.
+     rewrite size_empty nil_length Nat.sub_0_r.
+     iFrame.
+     iSplit; [iPureIntro; set_solver |].
+     done.
+   - iModIntro.
+     iIntros (hfuns fαs) "(%Hhfuns & %Hlen & HΨ & _)".
       wp_pures.
       wp_apply (wp_array_init (λ _ v, ⌜ v = #false ⌝%I)).
       + real_solver.
@@ -168,99 +291,384 @@ Section conc_bloom_filter.
         wp_pures.
         wp_alloc l as "Hl".
         wp_pures.
+        rewrite /Ψ.
+        iDestruct "HΨ" as "[%|(%s & Herr & %Hbound & Hfs)]";
+          [lia |].
+        iPoseProof (array.big_sepL_exists with "Hfs") as "(%hnames & Hfs)"; eauto.
         iApply "HΦ".
+        rewrite Hlen Nat.sub_diag Nat.mul_0_l.
+        iExists hfuns, a, hnames, s.
+        iAssert (([∗ list] v;x ∈ fαs;hnames, conhashfun x filter_size v ∗
+                ([∗ list] k ∈ ks, ∃ v0 : nat, ⌜v0 ∈ s⌝ ∗ hashkey x k (Some v0))) ∗
+                [∗ list] γ ∈ hnames, ([∗ set] k ∈ (set_seq 0 (S max_key) ∖ list_to_set ks),
+                  hashkey γ k None))%I with "[Hfs]" as "(?&?)".
+        { iApply (big_sepL2_sep_sepL_r _ _ fαs hnames).
+          iApply (big_sepL2_mono with "[$]").
+          iIntros (?????) "(?&?&?)".
+          iFrame. }
+        iFrame.
+        iMod (inv_alloc _ _ (bloom_filter_inv_aux l hfuns a hnames ks s) with "[-]") as "#Hinv";
+          [| iApply "Hinv"].
+        rewrite /bloom_filter_inv_aux.
         iModIntro.
-        iPoseProof (array.big_sepL_exists with "Hinvs") as "(%fs & Hinvs)"; auto.
-   Admitted.
+        iExists fαs.
+        iFrame.
+        iPureIntro.
+        repeat split; auto.
+        ** lia.
+        ** intros i Hi.
+           right.
+           pose proof (lookup_lt_is_Some_2 arr i) as [b Hb]; [lia |].
+           rewrite Hb.
+           apply Harr in Hb; auto.
+           by simplify_eq.
+        ** intros i Hi1 Hi2.
+           specialize (Harr i #true Hi2).
+           simplify_eq.
+ Qed.
 
-
-
-  Lemma bloom_filter_insert_thread_spec N bfl hfuns a fs αs ls hms hnames (s : gset nat) (x : nat) :
-    {{{ ([∗ set] x ∈ s, ∃ γ, (⌜ γ ∈ hnames ⌝∗ (hash_set_frag1 x γ.2.1))) ∗
-          bloom_filter_inv N bfl hfuns a fs αs ls hms hnames s
-    }}}
-      insert_bloom_filter #bfl #x
-      {{{ RET #(); True  }}}.
+  Lemma bloom_filter_insert_thread_spec N bfl hfuns a hnames (k : nat) (ks : list nat) s :
+    (k ∈ ks) ->
+    ([∗ list] k ∈ ks, ⌜ (k ≤ max_key)%nat ⌝) -∗
+    {{{ bloom_filter_inv N bfl hfuns a hnames ks s }}}
+      insert_bloom_filter #bfl #k
+    {{{ RET #(); True  }}}.
   Proof.
-    iIntros (Φ) "(Hs & #Hinv) HΦ".
-    rewrite /insert_bloom_filter /is_bloom_filter.
+    iIntros (Hk Hleq Φ) "!# #Hinv HΦ".
+    rewrite /insert_bloom_filter.
     wp_pures.
     wp_bind (! _)%E.
-    iInv "Hinv" as "(Hbfll&#Hfs&Hlen&Hnames&Hbound&?)" "Hclose".
+    iInv "Hinv" as "(%hfs&>Hbfl&>%Hhfs&>%Hlen&#Hhinv&>%Hbound&?)" "Hclose".
     wp_load.
-    iMod ("Hclose" with "[$]").
+    iMod ("Hclose" with "[-HΦ]").
+    {
+      iModIntro.
+      iExists hfs.
+      iFrame.
+      repeat iSplit; auto.
+    }
     iModIntro.
     wp_pures.
     wp_apply (wp_list_iter_invariant_HO
-               (λ l1 l2,
-                   ∃ hfuns2 fs2 αs2 ls2 hms2 hnames2,
-                     ⌜ l2 = (zip_with (λ v1 v2, PairV v1 v2) fs2 αs2) ⌝ ∗
-                   ( [∗ list] i ↦ α;γ ∈ αs2; hnames2, hash_tape_token α 1 γ.2.2.1 ) ∗
-                   con_hash_inv_list N fs2 αs2 ls2 hms2 hnames2)%I
-               with "[][][HΦ]"); auto.
-    - iIntros (lpre w lsuf Ψ).
-      iModIntro.
-      iIntros "(%Hlist & (%&%&%&%&%&%H&Htoks&Hiter)) HΨ".
-      destruct fs2 as [|f fs3], αs2 as [|α αs3]; simpl in H; try inversion H.
-      iPoseProof (con_hash_inv_list_cons with "Hiter") as
-        "(%α' & %αs3' & %lk & %lks3 & %hm & %hms3 & %γ & %hnames3 & (%Hα & -> & -> & -> & (%ns & Hht ) & Hinvcur & ?))".
-      inversion Hα; destruct Hα; simplify_eq.
-      iDestruct "Htoks" as "(Htok&Htoks)".
+                (λ fs1 fs2,
+                   ∃ hnames2,
+                    con_hash_inv_list fs2 hnames2 ks s)%I with "[][][HΦ]"); auto.
+    - iIntros (fs1 f fs2 Ψ) "!# (%hnames2 & Hiter) HΨ".
       wp_pures.
-      iPoseProof (hash_token_non_empty with "Hht Htok") as "(%n & %ns' & ->)".
-      wp_bind (f _ _)%E.
-      wp_apply (con_hash_spec_test1 with "[$Hinvcur $Hht]").
-      iIntros (res) "(Hfrag & [(Hht & ->)| Hht])".
-      + wp_pures.
-        iInv "Hinv" as "(?&?&?&?&?&(%arr&Harr&>%HlenA&?))" "Hclose".
-        iPoseProof (hash_frag_valid with "Hfrag") as "%".
-        wp_apply (wp_store_offset with "[$Harr]").
-        {
-          apply lookup_lt_is_Some_2.
-          rewrite HlenA //.
-          lia.
-        }
-        iIntros "Harr".
-        iMod ("Hclose" with "[-HΨ]").
-        {
-          iModIntro.
-          iFrame.
-          admit.
-        }
+      rewrite /con_hash_inv_list.
+      iPoseProof (con_hash_inv_list_cons with "Hiter")
+        as "(%γ&%hnames3&->&#Hinvf&Hfrags&Htail)".
+      wp_bind (f _).
+      iPoseProof (big_sepL_elem_of _ _ k with "Hfrags") as "(%v&%Hv&#Hfrag)"; auto.
+      wp_apply (wp_conhashfun_prev with "[$Hfrag //]").
+      iIntros "_".
+      wp_pures.
+      iInv "Hinv" as "(%&?&?&?&?&?&%arr&Harr&>%HlenA&>%Htf&>%Htrue)" "Hclose".
+      wp_apply (wp_store_offset with "[$Harr]").
+      {
+        apply lookup_lt_is_Some_2.
+        rewrite HlenA //.
+        by apply Hbound.
+      }
+      iIntros "Harr".
+      iMod ("Hclose" with "[-HΨ Htail]").
+      {
         iModIntro.
-        iApply "HΨ".
-        admit.
-      + wp_pures.
-        iInv "Hinv" as "(?&?&?&?&?&(%arr&Harr&>%HlenA&?))" "Hclose".
-        iPoseProof (hash_frag_valid with "Hfrag") as "%".
-        wp_apply (wp_store_offset with "[$Harr]").
-        {
-          apply lookup_lt_is_Some_2.
-          rewrite HlenA //.
-          lia.
-        }
-        iIntros "Harr".
-        iMod ("Hclose" with "[-HΨ]").
-        {
-          iModIntro.
-          iFrame.
-          admit.
-        }
-        iModIntro.
-        iApply "HΨ".
-        admit.
-   - iSplitL "Hfs".
-     { done. }
-     iExists _,fs,αs,ls,hms,hnames.
-     iFrame.
-     admit.
+        iFrame.
+        iPureIntro.
+        repeat split.
+        - rewrite insert_length //.
+        - intros i Hi.
+          destruct (decide (i = v)) as [-> | Hneq]; auto.
+          + rewrite list_lookup_insert; [auto|lia].
+          + rewrite list_lookup_insert_ne; auto.
+        - intros i Hi Hlookup.
+          destruct (decide (i = v)) as [-> | Hneq]; auto.
+          apply Htrue; auto.
+          by rewrite list_lookup_insert_ne in Hlookup.
+      }
+      iApply "HΨ".
+      iModIntro.
+      rewrite /con_hash_inv_list.
+      iExists hnames3.
+      iFrame.
    - iModIntro.
      iIntros "?".
      by iApply "HΦ".
-  Admitted.
+ Qed.
+
+ Lemma bloom_filter_lookup_spec N bfl hfuns a hnames (k : nat) (ks : list nat) s :
+    (k ∉ ks) ->
+    (k ≤ max_key)%nat ->
+    ([∗ list] k ∈ ks, ⌜ (k ≤ max_key)%nat ⌝) -∗
+    {{{ ↯ (fp_error filter_size num_hash 0 (size s)) ∗
+         ([∗ list] γ ∈ hnames, hashkey γ k None) ∗
+        bloom_filter_inv N bfl hfuns a hnames ks s }}}
+           lookup_bloom_filter #bfl #k
+      {{{ v, RET v; ⌜ v = #false ⌝ }}}.
+ Proof.
+   iIntros (Hk Hkleq Hksleq Φ) "!# (Herr & Hfrags & #Hinv) HΦ".
+   rewrite /lookup_bloom_filter.
+   wp_pures.
+   wp_bind (!_)%E.
+   iInv "Hinv" as "(%hfs&>Hbfl&>%Hhfs&>%Hlen&#Hhinv&>%Hbound&?)" "Hclose".
+   wp_load.
+   iMod ("Hclose" with "[-HΦ Herr Hfrags]").
+   {
+     iModIntro.
+     iExists hfs.
+     iFrame.
+     repeat iSplit; auto.
+   }
+   iModIntro.
+   wp_pures.
+   wp_alloc res as "Hres".
+   wp_pures.
+   wp_apply (wp_list_iter_invariant_HO
+               (λ fs1 fs2,
+                 (∃ hnames2,
+                     ([∗ list] γ ∈ hnames2, hashkey γ k None) ∗
+                     con_hash_inv_list fs2 hnames2 ks s) ∗
+                 (res ↦ #false ∨
+                 (res ↦ #true ∗
+                          ↯ ((size s / (filter_size + 1)) ^ (length fs2))%R)))%I
+              with "[][Hfrags Herr Hres][HΦ]").
+   - iIntros (fs1 f fs2 Ψ) "!# ((%γ2 & Hfrags & Hiter) & [Hr | (Hr & Herr)]) HΨ".
+     + wp_pures.
+       wp_bind (f _).
+       iPoseProof (con_hash_inv_list_cons with "Hiter")
+         as "(%γ&%hnames3&->&#Hinvf&HSome&Htail)".
+       iPoseProof (big_sepL_cons with "Hfrags") as "(?&Hfrags)".
+       wp_apply (wp_hash_lookup_safe with "[$]").
+       iIntros (v) "(%&#?)".
+       wp_pures.
+       wp_bind (!_)%E.
+       iInv "Hinv" as "(%&?&?&?&?&?&%arr&Harr&>%HlenA&>%Htf&>%Htrue)" "Hclose".
+       pose proof (lookup_lt_is_Some_2 arr v) as [x Hx]; [lia|].
+       wp_apply (wp_load_offset with "Harr"); eauto.
+       iIntros "Harr".
+       iMod ("Hclose" with "[- Hr HΨ Hfrags Htail]").
+       {
+         iModIntro.
+         iExists hfs.
+         iFrame.
+         repeat iSplit; auto.
+       }
+       iModIntro.
+       pose proof (Htf v) as [?|?]; [lia | |]; simplify_eq.
+       * wp_pures.
+         iModIntro.
+         iApply "HΨ".
+         iFrame.
+       * wp_pures.
+         wp_store.
+         iModIntro.
+         iApply "HΨ".
+         iFrame.
+
+     + wp_pures.
+       wp_bind (f _).
+       iPoseProof (con_hash_inv_list_cons with "Hiter")
+         as "(%γ&%hnames3&->&#Hinvf&HSome&Htail)".
+
+       iPoseProof (big_sepL_cons with "Hfrags") as "(Hknone&Hfrags)".
+       assert
+         (forall z, (0 <= (size s / (filter_size + 1))^z)%R) as Haux.
+       {
+         intro z.
+         apply pow_le.
+         apply Rcomplements.Rdiv_le_0_compat; real_solver.
+       }
+       wp_apply (wp_hash_lookup_avoid_set _ _ _ s
+                     (mknonnegreal _ (Haux (length (f :: fs2) )))
+                     (mknonnegreal _ (Haux (length fs2 )))
+                     0%NNR with "[$Herr $Hknone]"); auto.
+       {
+         simpl. rewrite Rmult_0_l Rplus_0_r.
+         rewrite -(Rmult_comm (filter_size + 1))
+            -Rmult_assoc
+            Rmult_div_assoc
+            Rmult_div_r; [lra |].
+         real_solver.
+       }
+       simpl.
+       iIntros (v) "(%Hv & [(%Hin & Herr) | (%Hout & Herr)] & Hksome)".
+       * wp_pures.
+         wp_bind (!_)%E.
+         iInv "Hinv" as "(%&?&?&?&?&?&%arr&Harr&>%HlenA&>%Htf&>%Htrue)" "Hclose".
+         pose proof (lookup_lt_is_Some_2 arr v) as [x Hx]; [lia|].
+         wp_apply (wp_load_offset with "Harr"); eauto.
+         iIntros "Harr".
+         iMod ("Hclose" with "[- Hr HΨ Hfrags Htail Herr]").
+         {
+           iModIntro.
+           iExists hfs.
+           iFrame.
+           repeat iSplit; auto.
+         }
+         iModIntro.
+         pose proof (Htf v) as [?|?]; [lia | |]; simplify_eq.
+         ** wp_pures.
+            iModIntro.
+            iApply "HΨ".
+            iFrame.
+            iRight; iFrame.
+         ** wp_pures.
+            wp_store.
+            iModIntro.
+            iApply "HΨ".
+            iFrame.
+       * wp_pures.
+         wp_bind (!_)%E.
+         iInv "Hinv" as "(%&?&?&?&?&?&%arr&Harr&>%HlenA&>%Htf&>%Htrue)" "Hclose".
+         assert (arr !! v = Some #false) as Hlookup.
+         {
+           pose proof (Htf v) as [H1 | H2]; [lia| |auto].
+           exfalso.
+           apply Hout, Htrue; auto.
+           lia.
+         }
+         wp_apply (wp_load_offset with "Harr"); eauto.
+         iIntros "Harr".
+         iMod ("Hclose" with "[- Hr HΨ Hfrags Htail]").
+         {
+           iModIntro.
+           iExists hfs.
+           iFrame.
+           repeat iSplit; auto.
+         }
+         iModIntro.
+         wp_pures.
+         wp_store.
+         iModIntro.
+         iApply "HΨ".
+         iFrame.
+
+  - iSplit; auto.
+    iSplitR "Hres Herr".
+    + iExists hnames.
+      auto.
+    + iRight.
+      iFrame.
+      rewrite /fp_error Hlen.
+      case_bool_decide; [|iFrame].
+      iPoseProof (ec_contradict with "Herr") as "?"; auto.
+      simpl; lra.
+  - iModIntro.
+    iIntros "((%hnames2 & ? & ?)&[Hres | (Hres & Herr)])".
+    * wp_pures.
+      wp_load.
+      by iApply "HΦ".
+    * simpl.
+      iPoseProof (ec_contradict with "Herr") as "?"; auto; lra.
+ Qed.
 
 
+  Lemma insert_bloom_filter_loop_spec N bfl hfuns a hnames s
+          (ns ks : list nat) (ksv : val) :
+    is_list ks ksv ->
+    {{{ bloom_filter_inv N bfl hfuns a hnames ns s ∗
+        ([∗ list] k ∈ ks, ⌜k ∈ ns ⌝) ∗
+        ([∗ list] k ∈ ns, ⌜ (k ≤ max_key)%nat ⌝)
+    }}}
+      insert_bloom_filter_loop #bfl ksv
+    {{{ v, RET v; True }}}.
+  Proof.
+    iIntros (Hksv Φ) "(#Hinv & %Hks & %Hns) HΦ".
+    rewrite /insert_bloom_filter_loop.
+    iInduction ks as [|k ks'] "IH" forall (ksv Hksv Φ).
+    - simpl in Hksv.
+      simplify_eq.
+      wp_pures.
+      by iApply "HΦ".
+    - destruct Hksv as [kv [-> Htail]].
+      wp_pures.
+      simpl.
+      wp_apply (wp_par (λ _, True)%I (λ _, True)%I).
+      + wp_apply (bloom_filter_insert_thread_spec _ _ _ _ _ _ ns); auto.
+        apply (Hks 0); auto.
+      + iSpecialize ("IH" with "[]").
+        {
+          iPureIntro.
+          intros i ? ?.
+          apply (Hks (S i)).
+          auto.
+        }
+        iApply "IH"; auto.
+      + iIntros (? ?) "? !>".
+        by iApply "HΦ".
+  Qed.
+
+
+  Lemma insert_bloom_filter_loop_seq_spec N bfl hfuns a hnames s
+          (ns ks : list nat) (ksv : val) :
+    is_list ks ksv ->
+    {{{ bloom_filter_inv N bfl hfuns a hnames ns s ∗
+        ([∗ list] k ∈ ks, ⌜k ∈ ns ⌝) ∗
+        ([∗ list] k ∈ ns, ⌜ (k ≤ max_key)%nat ⌝)
+    }}}
+      insert_bloom_filter_loop_seq #bfl ksv
+    {{{ v, RET v; True }}}.
+  Proof.
+    iIntros (Hksv Φ) "(#Hinv & %Hks & %Hns) HΦ".
+    rewrite /insert_bloom_filter_loop_seq.
+    iInduction ks as [|k ks'] "IH" forall (ksv Hksv Φ).
+    - simpl in Hksv.
+      simplify_eq.
+      wp_pures.
+      by iApply "HΦ".
+    - destruct Hksv as [kv [-> Htail]].
+      wp_pures.
+      simpl.
+      wp_bind (insert_bloom_filter _ _).
+      wp_apply (bloom_filter_insert_thread_spec _ _ _ _ _ _ ns); auto.
+      { apply (Hks 0); auto. }
+      iIntros "_".
+      do 2 wp_pure.
+      iSpecialize ("IH" with "[]").
+      {
+        iPureIntro.
+        intros i ? ?.
+        apply (Hks (S i)).
+        auto.
+      }
+      iApply "IH"; auto.
+  Qed.
+
+ Lemma main_bloom_filter_seq_spec (N : namespace) (ks : list nat) (ksv : val) (ktest : nat) :
+      NoDup ks ->
+      is_list ks ksv ->
+      ktest ∉ ks ->
+      (ktest ≤ max_key)%nat ->
+      {{{ ([∗ list] k ∈ ks, ⌜ (k ≤ max_key)%nat ⌝) ∗
+           ↯ (fp_error filter_size num_hash (num_hash * length ks) 0) }}}
+        main_bloom_filter_seq ksv #ktest
+      {{{ v, RET v; ⌜ v = #false ⌝ }}}.
+ Proof.
+   iIntros (Hndup Hksv Hktest Htestvalid Φ) "(#Hks & Herr) HΦ".
+   rewrite /main_bloom_filter_seq.
+   wp_apply (bloom_filter_init_spec N ks with "[//] Herr"); auto.
+   iIntros (bfl) "(%hfuns & %a & %hnames & %s & Herr & Hauths & #Hinv)".
+   wp_pures.
+   wp_apply (insert_bloom_filter_loop_seq_spec N _ _ _ _ _ ks ks); auto.
+   {
+     repeat iSplit; auto.
+     iPureIntro.
+     intros ? ? ?.
+     simpl.
+     eapply elem_of_list_lookup_2; eauto.
+   }
+   iIntros (?) "_".
+   wp_pures.
+   wp_apply (bloom_filter_lookup_spec N _ _ _ hnames _ ks s with "[][Herr Hauths]"); auto.
+   iFrame.
+   iSplit; auto.
+   iApply (big_sepL_mono with "Hauths").
+   iIntros (k γ Hk) "Hnones".
+   iApply (big_sepS_elem_of with "Hnones").
+   apply elem_of_difference; split.
+   - apply elem_of_set_seq; split; lia.
+   - by apply not_elem_of_list_to_set.
+ Qed.
 
 End conc_bloom_filter.
-
-*)
